KLR/Semantics/ProofRules.lean
@@ -324,7 +324,7 @@ theorem wpResync : ⊢ Φ p1 p2 -∗ dwp 0 0 Lx Rx p1 p2 Φ := by
 
 -- NB. Keeping this code in the repo as an example for writing basic proof rules.
 /-- `dwp` for a single pure step on the left. -/
-theorem dwpPureL (Hstep : PureStep p1 p1') (Hx : 0 < Lx := by omega) :
+theorem dwpPureL (Hstep : SPure p1 p1' HP) (H : HP) (Hx : 0 < Lx := by omega) :
     ⊢ dwp (Lm - 1) Rm (Lx - 1) Rx p1' p2 Φ -∗ dwp Lm Rm Lx Rx p1 p2 Φ := by
   -- Unfold the dwp
   unfold dwp
@@ -348,14 +348,14 @@ theorem dwpPureL (Hstep : PureStep p1 p1') (Hx : 0 < Lx := by omega) :
     ipure_intro
     obtain ⟨_, _, _, _, _, _⟩ := Hstep
     refine ⟨?_, ?_, ?_, ?_, ?_, ?_⟩ <;> try omega
-    refine StepN.step (Hstep sl) ?_
+    refine StepN.step (Hstep sl H) ?_
     trivial
   · iexact Hstate
 
 
 -- NB. Keeping this code in the repo as an example for writing basic proof rules.
 /-- `dwp` for a single pure step on the right. -/
-theorem dwpPureR (Hstep : SmallStep.PureStep p2 p2') (Hx : 0 < Rx := by omega) :
+theorem dwpPureR (Hstep : SPure p2 p2' HP) (H : HP) (Hx : 0 < Rx := by omega) :
     ⊢ dwp Lm (Rm - 1) Lx (Rx - 1) p1 p2' Φ -∗ dwp Lm Rm Lx Rx p1 p2 Φ := by
   -- Unfold the dwp
   unfold dwp
@@ -379,9 +379,13 @@ theorem dwpPureR (Hstep : SmallStep.PureStep p2 p2') (Hx : 0 < Rx := by omega) :
     ipure_intro
     obtain ⟨_, _, _, _, _, _⟩ := Hstep
     refine ⟨?_, ?_, ?_, ?_, ?_, ?_⟩ <;> try omega
-    refine StepN.step (Hstep sr) ?_
+    refine StepN.step (Hstep sr H) ?_
     trivial
   · iexact H
+
+
+
+
 
 
 
@@ -517,8 +521,9 @@ theorem dwpAllocR (Hx : 1 < Rx := by omega) :
         exact step.asnV
       · exact SR
   · iexact H
+-/
 
-
+/-
 theorem dwpSetpL {v : DataT} (Hx : 0 < Lx := by omega) :
     ⊢ ((⟨i, x⟩ ↦ₗ some v) -∗ dwp (Lm - 1) Rm (Lx - 1) Rx (.run <| p1) p2 Φ) -∗
        (⟨i, x⟩ ↦ₗ mv) -∗
@@ -558,28 +563,59 @@ theorem dwpSetpL {v : DataT} (Hx : 0 < Lx := by omega) :
   refine ⟨?_, ?_, ?_, ?_, ?_, ?_⟩ <;> try omega
   rw [Nat.add_comm _ _, StepN_add_iff]
   refine ⟨_, ⟨stepN_1_iff_step.mpr step.setp, SL⟩⟩
+-/
 
-
-theorem dwpSetpL' {v : DataT} (Hx : 0 < Lx := by omega) :
-    ((⟨i, x⟩ ↦ₗ mv) ∗ ((⟨i, x⟩ ↦ₗ some v) -∗ dwp (Lm - 1) Rm (Lx - 1) Rx (.run <| p1) p2 Φ))
-    ⊢ (dwp Lm Rm Lx Rx (.run <| ⟨.setp (.val <| .uptr i) (.val <| .iptr x) (.val <| .data v), loc⟩ :: p1) p2 Φ) := by
-  apply BI.wand_entails
-  refine .trans (@dwpSetpL DataT Lx i x Lm Rm Rx p1 p2 Φ mv loc v Hx) ?_
-  iintro H1 ⟨H2, H3⟩
-  iapply H1 with [H3]
-  iexact H2
+theorem dwpSetpL {v : DataT} (Hx : 0 < Lx := by omega) :
+    ((⟨i, x⟩ ↦ₗ mv) ∗ ((⟨i, x⟩ ↦ₗ some v) -∗ dwp (Lm - 1) Rm (Lx - 1) Rx (.run p1 loc) p2 Φ))
+    ⊢ (dwp Lm Rm Lx Rx (.run (.setp (.val <| .uptr i) (.val <| .iptr x) (.val <| .data v) :: p1) loc) p2 Φ) := by
+  -- Unfold the dwp in the conclusion
+  iintro ⟨Hmv, Hdwp⟩
+  conv => rhs; unfold dwp
+  iintro sl sr Hs
+  refine include_sep (@update_set_lemma_left DataT ⟨i, x⟩ sl sr mv (some v)) ?_
+  -- Add the update lemma to the context
+  iintro ⟨Hupd, ⟨Hmv, Hdqp⟩, Hσ⟩
+  ispecialize Hupd Hmv Hσ
+  -- Eliminate bupds from the hypotheses but not the conclusion, by duplicating the bupd in the conclusion.
+  istop
+  refine .trans ?_ bupd_idem.mp
+  refine .trans bupd_frame_l (BIUpdate.mono ?_)
+  iintro ⟨Hdwp, ⟨Hfrac, Hauth⟩⟩
+  -- Specialize, unfold, and specialize the dwp
+  ispecialize Hdwp Hfrac
+  unfold dwp
+  ispecialize Hdwp _ sr Hauth
+  -- Eliminate the bupd
+  refine .trans emp_sep.mp (BIUpdate.mono ?_)
+  -- Conclude using the current hypotheses
+  iintro ⟨p1', p2', HΦ, s1, s2, ⟨n1, n2, %Hstep⟩, H⟩
+  iexists p1'
+  iexists p2'
+  isplit l [HΦ]
+  · iexact HΦ
+  iexists s1
+  iexists s2
+  isplit r [H] <;> try iexact H
+  iexists (n1 + 1)
+  iexists n2
+  ipure_intro
+  obtain ⟨_, _, _, _, SL, _⟩ := Hstep
+  refine ⟨?_, ?_, ?_, ?_, ?_, ?_⟩ <;> try omega
+  rw [Nat.add_comm _ _, StepN_add_iff]
+  refine ⟨_, ⟨stepN_1_iff_step.mpr ?_, SL⟩⟩
+  simp only [Step, NML.step]
+  congr
 
 theorem dwpSetpR {v : DataT} (Hx : 0 < Rx := by omega) :
-    ⊢ ((⟨i, x⟩ ↦ᵣ some v) -∗ dwp Lm (Rm - 1) Lx (Rx - 1) p1 (.run <| p2) Φ) -∗
-       (⟨i, x⟩ ↦ᵣ mv) -∗
-       (dwp Lm Rm Lx Rx p1 (.run <| ⟨.setp (.val <| .uptr i) (.val <| .iptr x) (.val <| .data v), loc⟩ :: p2) Φ) := by
+    ((⟨i, x⟩ ↦ᵣ mv) ∗ ((⟨i, x⟩ ↦ᵣ some v) -∗ dwp Lm (Rm - 1) Lx (Rx - 1) p1 (.run p2 loc) Φ))
+    ⊢ (dwp Lm Rm Lx Rx p1 (.run (.setp (.val <| .uptr i) (.val <| .iptr x) (.val <| .data v) :: p2) loc) Φ) := by
   -- Unfold the dwp in the conclusion
-  iintro Hdwp
+  iintro ⟨Hmv, Hdwp⟩
   conv => rhs; unfold dwp
-  iintro Hmv sl sr Hs
+  iintro sl sr Hs
   -- Add the update lemma to the context
   refine include_sep (@update_set_lemma_right DataT ⟨i, x⟩ sl sr mv (some v)) ?_
-  iintro ⟨Hupd, ⟨Hdwp, Hmv⟩, Hσ⟩
+  iintro ⟨Hupd, ⟨Hmv, Hdwp⟩, Hσ⟩
   ispecialize Hupd Hmv Hσ
   -- Eliminate bupds from the hypotheses but not the conclusion, by duplicating the bupd in the conclusion.
   istop
@@ -607,18 +643,16 @@ theorem dwpSetpR {v : DataT} (Hx : 0 < Rx := by omega) :
   obtain ⟨_, _, _, _, _, SR⟩ := Hstep
   refine ⟨?_, ?_, ?_, ?_, ?_, ?_⟩ <;> try omega
   rw [Nat.add_comm _ _, StepN_add_iff]
-  refine ⟨_, ⟨stepN_1_iff_step.mpr step.setp, SR⟩⟩
-
-theorem dwpSetpR' {v : DataT} (Hx : 0 < Rx := by omega) :
-    ((⟨i, x⟩ ↦ᵣ mv) ∗ ((⟨i, x⟩ ↦ᵣ some v) -∗ dwp Lm (Rm - 1) Lx (Rx - 1) p1 (.run <| p2) Φ))
-    ⊢ (dwp Lm Rm Lx Rx p1 (.run <| ⟨.setp (.val <| .uptr i) (.val <| .iptr x) (.val <| .data v), loc⟩ :: p2) Φ) := by
-  apply BI.wand_entails
-  refine .trans (@dwpSetpR DataT Rx i x Lm Rm Lx p1 p2 Φ mv loc v Hx) ?_
-  iintro H1 ⟨H2, H3⟩
-  iapply H1 with [H3]
-  iexact H2
+  refine ⟨_, ⟨stepN_1_iff_step.mpr ?_, SR⟩⟩
+  simp only [Step, NML.step]
+  congr
 
 
+
+
+
+
+/-
 -- TODO: This is only used for an example right now, a less ad-hoc solution for
 -- ExprSteps that use state is necessary.
 theorem dwpReadpRetL {v : DataT} (Hx : 0 < Lx := by omega) :
@@ -722,7 +756,7 @@ theorem dwpLoopDoneR (Hx : 1 < Rx := by omega) :
     exact step.loop_exit
   · iexact Hσ
 
-
+-/
 
 -- /- Proposition over locals. Used for generalization.
 -- LocProp should be solvable by `simp` for good automation. -/
@@ -734,16 +768,14 @@ theorem dwpLoopDoneR (Hx : 1 < Rx := by omega) :
 
 
 /-- Generalize a wp by a relationship on its locations -/
-theorem wp_gen_loc (R : Locals DataT → Locals DataT → Prop) :
-  ⊢ (∀ locₗ locᵣ, ⌜R locₗ locᵣ⌝ -∗ wp (DataT := DataT) K (.run <| ⟨sₗ, locₗ⟩ :: pₗ) (.run <| ⟨sᵣ, locᵣ⟩ :: pᵣ) Φ) -∗
+theorem wp_gen_loc (R : LocalContext DataT → LocalContext DataT → Prop) :
+  ⊢ (∀ locₗ locᵣ, ⌜R locₗ locᵣ⌝ -∗ wp (DataT := DataT) K (.run (sₗ :: pₗ) locₗ) (.run (sᵣ :: pᵣ) locᵣ) Φ) -∗
     ⌜R llₗ llᵣ⌝ -∗
-    wp (DataT := DataT) K (.run <| ⟨sₗ, llₗ⟩ :: pₗ) (.run <| ⟨sᵣ, llᵣ⟩ :: pᵣ) Φ := by
+    wp (DataT := DataT) K (.run (sₗ :: pₗ) llₗ) (.run (sᵣ :: pᵣ) llᵣ) Φ := by
   iintro H HR
   ispecialize H _ _ HR
   iexact H
 
-
--/
 
 end dwp
 
@@ -786,8 +818,9 @@ open Iris Iris.BI Iris.BI.BIBase KLR.Core Iris NML SmallStep
 
 variable {DataT : Type _}
 
+-- TODO: Inline into dwpL
 /-- Step the left-hand side of a dwp using a `uwpL`. -/
-theorem dwpL (u : uwpL DataT) (Hx : u.steps ≤ Lx) :
+theorem dwpL' (u : uwpL DataT) (Hx : u.steps ≤ Lx) :
     ⊢ u.pre ∗ (u.post -∗ dwp (Lm - u.steps) Rm (Lx - u.steps) Rx u.prog' pr Φ)  -∗
       dwp Lm Rm Lx Rx u.prog pr Φ := by
   -- Include the spec inside the separating context
@@ -827,13 +860,13 @@ theorem dwpL (u : uwpL DataT) (Hx : u.steps ≤ Lx) :
     exists (u.prog', sl')
   · iexact Hs''
 
--- Let's see if this even works before going ham with the refactoring
-theorem dwpL' (u : uwpL DataT) (Hx : u.steps ≤ Lx) :
+theorem dwpL (u : uwpL DataT) (Hx : u.steps ≤ Lx) :
     u.pre ∗ (u.post -∗ dwp (Lm - u.steps) Rm (Lx - u.steps) Rx u.prog' pr Φ) ⊢
-    dwp Lm Rm Lx Rx u.prog pr Φ := (wand_entails <| dwpL u Hx)
+    dwp Lm Rm Lx Rx u.prog pr Φ := (wand_entails <| dwpL' u Hx)
 
+-- TODO: Inline into dwpR
 /-- Step the right-hand side of a dwp using a `uwpR`. -/
-theorem dwpR (u : uwpR DataT) (Hx : u.steps ≤ Rx) :
+theorem dwpR' (u : uwpR DataT) (Hx : u.steps ≤ Rx) :
     ⊢ u.pre ∗ (u.post -∗ dwp Lm (Rm - u.steps) Lx (Rx - u.steps) pl u.prog' Φ) -∗
       dwp Lm Rm Lx Rx pl u.prog Φ := by
   -- Include the spec inside the separating context
@@ -873,13 +906,12 @@ theorem dwpR (u : uwpR DataT) (Hx : u.steps ≤ Rx) :
     exists (u.prog', sr')
   · iexact Hs''
 
--- Let's see if this even works before going ham with the refactoring
-theorem dwpR' (u : uwpR DataT) (Hx : u.steps ≤ Rx) :
+theorem dwpR (u : uwpR DataT) (Hx : u.steps ≤ Rx) :
     u.pre ∗ (u.post -∗ dwp Lm (Rm - u.steps) Lx (Rx - u.steps) pl u.prog' Φ)
     ⊢ dwp Lm Rm Lx Rx pl u.prog Φ :=
-  (wand_entails <| dwpR u Hx)
+  (wand_entails <| dwpR' u Hx)
 
-@[simp] def uwpPureL {p p' : Prog DataT} (H : PureStep p p') : uwpL DataT where
+@[simp] def uwpPureL {p p' : Prog DataT} (H : SPure p p' H') (HH' : H') : uwpL DataT where
   pre   := iprop(True)
   post  := iprop(True)
   prog  := p
@@ -890,13 +922,13 @@ theorem dwpR' (u : uwpR DataT) (Hx : u.steps ≤ Rx) :
     iexists σₗ
     isplit r
     · ipure_intro
-      exact stepN_1_iff_step.mpr <| H σₗ
+      exact stepN_1_iff_step.mpr <| H σₗ HH'
     · refine .trans ?_ BIUpdate.intro
       refine .trans ?_ sep_true.mpr
       iintro Hσ
       iexact Hσ
 
-@[simp] def uwpPureR {p p' : Prog DataT} (H : PureStep p p') : uwpR DataT where
+@[simp] def uwpPureR {p p' : Prog DataT} (H : SPure p p' H') (HH' : H') : uwpR DataT where
   pre   := iprop(True)
   post  := iprop(True)
   prog  := p
@@ -907,7 +939,7 @@ theorem dwpR' (u : uwpR DataT) (Hx : u.steps ≤ Rx) :
     iexists σᵣ
     isplit r
     · ipure_intro
-      exact stepN_1_iff_step.mpr <| H σᵣ
+      exact stepN_1_iff_step.mpr <| H σᵣ HH'
     · refine .trans ?_ BIUpdate.intro
       refine .trans ?_ sep_true.mpr
       iintro Hσ
@@ -925,31 +957,6 @@ def uwpSetpL {i : ChipIndex} {x : Nat × Nat} {mv : Option DataT} {v : DataT} {l
   spec  := by
     sorry
 -/
-
-
-
--- | load_full :
---     AffineMap.is_trivial asn →
---     ExprStep e loc st (.ptr tensor) st' →
---     -- The source tensor must have index in HBM (can be generalized), and be allocated
---     tensor.index = ChipIndex.hbmIndex src_index →
---     ChipMemory.get_store st'.memory tensor.index = some src_store →
---     -- The destination tensor is a fresh tensor in SBUF, with updated state.
---     ⟨dst_index, memory''⟩ = ChipMemory.freshSBUFStore st'.memory →
---     ExprStep (.load asn e) loc st
---       -- Return value: The input tensor, but with its chip index updated to be the fresh tensor.
---       -- All other metadata is the same.
---       (.ptr {tensor with index := dst_index })
---       -- Return state: Update the SBUF state at the fresh index to contain the source store.
---       (State.mk <| ChipMemory.set_store memory'' dst_index (some src_store))
-
-
--- Next up:
--- Desync'd Moving tensors (load_full)
--- Sync'd Control flow (iterators as values)
--- Desync'd tensorscalar
--- Sync'd ret_assert
--- This should be enought to verify loop fusion
 
 end uwp
 
@@ -1082,10 +1089,6 @@ structure ewpR (DataT : Type _) extends ewp DataT where
 
 
 
-
-
--- NTS: Not sure I want to do sbuf_alloc in this format because the expression returned it depends on state
--- But you should add set or something to make sure it works
 
 
 end ewp
